%\begin{figure}[h]
\subsubsection*{Precedes(e$_1$,e$_2$):}
\begin{eplpseudocode}
$\llbracket$Precedes(e$_1$,e$_2$)$\rrbracket$=WindowIfComplex($\llbracket$e$_1$$\rrbracket$) $\rightarrow$ WindowIfComplex($\llbracket$e$_2$$\rrbracket$) and not WindowIfComplex($\llbracket$e$_1$$\rrbracket$) 
\end{eplpseudocode}
%\(Precedes(E_1,E_2)(t)=(\exists t_1)(\forall t_2)(E_1(t_1)\wedge E_2(t)\wedge (t_1<t)\wedge ((t_1<t_2\leq t)\rightarrow \thicksim E_1(t_2)\vee \thicksim E_2(t_2)))\)\\

\(Precedes(E_1,E_2)(t)=(\exists t_1)(\forall t_2)(E_1(t_1)\wedge \thicksim E_1(t) \wedge E_2(t)\wedge (t_1<t)\wedge ((t_1<t_2<t)\rightarrow \thicksim (E_1(t_2)\vee E_2(t_2))))\)\\

$Followed$-\(by(E_1,And\)-\(not(First(E_2),E_1))(t)\)

\(First(E_2)(t)=(\forall t_1)(E_2(t)\wedge ((t_1<t)\rightarrow \thicksim E_2(t_1)))\)

$And$-\(not(First(E_2),E_1)(t)=(\forall t_1)(\thicksim E_1(t)\wedge E_2(t)\wedge ((t_1<t)\rightarrow \thicksim (E_1(t_1)\vee E_2(t_1))))\)

$Followed$-\(by(E_1,And\)-\(not(First(E_2),E_1))(t)=(\exists t_1)(\forall t_2)(E_1(t_1)\wedge \thicksim E_1(t) \wedge E_2(t)\wedge (t_1<t)\wedge ((t_1<t_2<t)\rightarrow \thicksim (E_1(t_2)\vee E_2(t_2))))\)\\

\subsubsection*{During(e,s):}
\begin{eplpseudocode}
$\llbracket$During(e,s)$\rrbracket$=Becomes($\llbracket$s$\rrbracket$,v$_{sb}$) $\rightarrow$ ( every $\llbracket$e$\rrbracket$ ) and not Becomes($\llbracket$s$\rrbracket$,v$_{se}$)
\end{eplpseudocode}
\(During(E,E_{sb},E_{se})(t)=(\exists t_1)(\forall t_2)(E_{sb}(t_1)\wedge \thicksim E_{se}(t)\wedge E(t)\wedge (t_1<t)\wedge ((t_1<t_2< t)\rightarrow \thicksim E_{se}(t_2)))\)\\


$Followed$-\(by(E_{sb},And\)-\(not(Every(E),E_{se}))(t)\)

\(Every(E)(t)=E(T)\)

$And$-\(not(Every(E),E_{se})(t)=(\forall t_1)(\thicksim E_{se}(t)\wedge E(t)\wedge ((t_1<t)\rightarrow \thicksim (E_{se}(t_1)))\)

$Followed$-\(by(E_{sb},And\)-\(not(Every(E),E_{se}))(t)=(\exists t_1)(\forall t_2)(E_{sb}(t_1)\wedge \thicksim E_{se}(t)\wedge E(t)\wedge (t_1<t)\wedge ((t_1<t_2<t)\rightarrow \thicksim E_{se}(t_2)))\)\\

\subsubsection*{Overlapping(s$_1$,s$_2$):}
\begin{eplpseudocode}
$\llbracket$Overlapping(s$_1$,s$_2$)$\rrbracket$=Becomes($\llbracket$s$_1$$\rrbracket$,v$_{s_{1}b}$) $\rightarrow$ Becomes($\llbracket$s$_2$$\rrbracket$,v$_{s_{2}b}$) and not Becomes($\llbracket$s$_1$$\rrbracket$,v$_{s_{1}e}$)$ \rightarrow$ 
                                                Becomes($\llbracket$s$_1$$\rrbracket$,v$_{s_{1}e}$) and not Becomes($\llbracket$s$_2$$\rrbracket$,v$_{s_{2}e}$) 
\end{eplpseudocode}
\(Overlapping(E_{s_{1}b},E_{s_{1}e},E_{s_{2}b},E_{s_{2}e})(t)=(\exists t_1)(\exists t_2)(\forall t_3)(E_{s_{1}b}(t1)\wedge \thicksim E_{s_{1}e}(t_2)\wedge E_{s_{2}b}(t2)\wedge \thicksim E_{s_{2}e}(t) \wedge E_{s_{1}e}(t)\wedge (t_1<t_2<t)\wedge ((t_1<t_3\leq t_2)\rightarrow \thicksim E_{s_{1}e}(t_3)) \wedge ((t_2<t_3\leq t)\rightarrow \thicksim E_{s_{2}e}(t_3))) \)\\

\subsubsection*{Occurs(e,s):}
\begin{eplpseudocode}
$\llbracket$Occurs(e,s)$\rrbracket$=Becomes($\llbracket$s$\rrbracket$,v) $\rightarrow$ ( every-distinct(timestamp) $\llbracket$e$\rrbracket$ ) and not Becomes($\llbracket$s$\rrbracket$,v')
\end{eplpseudocode}
\(Occurs(E,E_{sb},E_{se})(t)=(\exists t_1)(\forall t_2)(E_{sb}(t_1)\wedge E(t)\wedge (t_1<t)\wedge ((t_1<t_2<t)\rightarrow \thicksim E_{se}(t_2) \vee \thicksim E(t_2)))\)\\

\subsubsection*{Occurs(s$_1$,s$_2$):}
\begin{eplpseudocode}
$\llbracket$Occurs(s$_1$,s$_2$)$\rrbracket$=((Becomes($\llbracket$s$_1$$\rrbracket$,v) $\rightarrow$ every-distinct(timestamp) Becomes($\llbracket$s$_2$$\rrbracket$,v) and not Becomes($\llbracket$s$_1$$\rrbracket$,v'))
                  or 
                  (Becomes($\llbracket$s$_2$$\rrbracket$,v) $\rightarrow$ every-distinct(timestamp) Becomes($\llbracket$s$_1$$\rrbracket$,v) and not Becomes($\llbracket$s$_2$$\rrbracket$,v')))
\end{eplpseudocode}
\begin{eplpseudocode}
$\llbracket$Occurs(s$_1$,s$_2$)$\rrbracket$=Occurs(Becomes($\llbracket$s$_2$$\rrbracket$,v),$\llbracket$s$_1\rrbracket$)
                 or 
                 Occurs(Becomes($\llbracket$s$_1$$\rrbracket$,v),$\llbracket$s$_2\rrbracket$)
\end{eplpseudocode}
\(Occurs(E_{s_{1}b},E_{s_{1}2},E_{s_{2}b},E_{s_{2}e})(t)=(\exists t_1)(\forall t_2)((E_{s_{1}b}(t_1)\wedge E_{s_{2}b}(t)\wedge ((t_1<t_2<t)\rightarrow \thicksim E_{s_{1}e}(t_2)) \wedge ((t_1<t_2<t)\rightarrow \thicksim E_{s_{2}b}(t_2)))\vee (E_{s_{2}b}(t_1)\wedge E_{s_{1}b}(t)\wedge ((t_1<t_2<t)\rightarrow \thicksim E_{s_{2}e}(t_2)) \wedge ((t_1<t_2<t)\rightarrow \thicksim E_{s_{1}b}(t_2)))  \wedge (t_1<t))\)\\

\(Occurs(E_{s_{1}b},E_{s_{1}e},E_{s_{2}b},E_{s_{2}e})(t)=Occurs(E_{s_{2}b},E_{s_{1}b},E_{s_{1}e})(t)\vee Occurs(E_{s_{1}b},E_{s_{2}b},E_{s_{2}e})(t) \)\\

\subsubsection*{And(e$_0$,$\dots$,e$_n$):}
\begin{eplpseudocode}
$\llbracket$And(e$_1$, $\dots$ ,e$_n$)$\rrbracket$=WindowIfComplex($\llbracket$e$_1$$\rrbracket$) and $\dots$ and WindowIfComplex($\llbracket$e$_n$$\rrbracket$)
\end{eplpseudocode}
\(And(E_1, \dots , E_n)(t)=(\exists t_{i=1;n})(\exists i_0)(\forall t')(E_1(t_1)\underset{i}\wedge E_i(t_i) \wedge E_n(t_n)\wedge (t_1\leq t)\underset{i}\wedge (t_i\leq t) \wedge (t_n\leq t)\wedge (t_{i_0}=t) \wedge ((t'<t)\rightarrow \thicksim E_{i_0}(t')))\)\\

\subsubsection*{Or(e$_0$,$\dots$,e$_n$):}
\begin{eplpseudocode}
$\llbracket$Or(e$_1$, $\dots$ ,e$_n$)$\rrbracket$=WindowIfComplex($\llbracket$e$_1$$\rrbracket$) or $\dots$ or WindowIfComplex($\llbracket$e$_n$$\rrbracket$)
\end{eplpseudocode}
\(Or(E_0, \dots , E_n)(t)=E_0(t)\vee \dots \vee E_n(t)\)

%\end{figure}